playground/uart_model/m0u_progScript.sml
@@ -1,0 +1,228 @@
+open HolKernel Parse boolLib bossLib;
+open uartTheory
+open progTheory 
+open set_sepTheory
+open m0_NITTheory
+open uartTheory
+open clockTheory
+open stateTheory m0_stepTheory
+open boolSimps
+open pred_setTheory
+
+val _ = new_theory "m0u_prog";
+(********************************************)
+(*           UART separation logic          *)
+(*                                          *)
+(********************************************)
+
+val _= Datatype `m0u_component = m0_c m0_component
+                               | m0u_c_Input 
+                               | m0u_c_Output
+                               | m0u_c_RXD
+                               | m0u_c_TXD
+                               | m0u_c_RXDRDY
+                               | m0u_c_TXDRDY`;
+
+val _= Datatype `m0u_data = m0_d m0_data
+                          | m0u_d_stream (word32 list)
+                          | m0u_d_word32 word32
+                          | m0u_d_bool bool`;
+
+
+val m0u_proj_def = Define `
+m0u_proj ((s,u),input,output) =
+     (λa.
+         case a of
+	   m0_c b => m0_d (m0_proj s b)
+         | m0u_c_Input => m0u_d_stream input
+	 | m0u_c_Output => m0u_d_stream output
+         | m0u_c_RDX => m0u_d_word32 u.RXD
+         | m0u_c_TXD => m0u_d_word32 u.TXD
+         | m0u_c_RDXRDY => m0u_d_bool u.TXDRDY
+         | m0u_c_TXDRDY => m0u_d_bool u.RXDRDY) 
+`; 
+       
+(* Translate M0 separation logit to M0U separation logic *)  
+
+val TO_M0U_def = Define`
+ TO_M0U = IMAGE (m0_c ## m0_d )
+`;
+
+val TO_M0U_def = Define`
+ TO_M0U_PROP= IMAGE TO_M0U
+`;
+
+(********************************************)
+(*        Sep logic Domain theory           *)
+(********************************************)
+val r2m0_c_set_def = Define`
+r2m0_c_set region = IMAGE m0_c_MEM region
+`;
+
+val m0_SDOM_def = Define`
+SDOM A = (BIGUNION (IMAGE (IMAGE (\(c,_).c)) A)) `;
+
+val m0_SEP_INV_UNDER_NON_R_EQ_thm = prove(
+``!P region s s'. DISJOINT (SDOM P) (r2m0_c_set region) 
+    /\ SEP_REFINE (P * SEP_T) $= (STATE m0_proj) s 
+    /\ m0_non_r_eq region s s' ==>
+	SEP_REFINE (P * SEP_T) $= (STATE m0_proj) s'``,
+cheat);
+
+(********************************************)
+(*          Uart model prog                 *)
+(*                                          *)
+(********************************************)
+val NextStateM0U_def = Define ` NextStateM0U ((s0,u0),I0,O0) =
+      (let
+        ((s1,u1),I1,O1)  = m0u_Next ((s0,u0),I0,O0)
+      in
+          if (~u1.unpredictable /\ (s1.exception = NoException))
+         then SOME ((s1,u1),I1,O1) else NONE)`;
+
+val M0U_MODEL = Define `M0U_MODEL = (
+    STATE m0u_proj,
+    NEXT_REL $= NextStateM0U,(\c. TO_M0U (m0_instr c)),
+    $=  :((m0_state # uart_state) # word32 list # word32 list)-> 
+         ((m0_state # uart_state) # word32 list # word32 list)-> bool,
+    K F :((m0_state # uart_state) # word32 list # word32 list)-> bool
+    )`;
+
+val COSIM_def = Define ` COSIM P t = ! s s' seq seq' i.   
+    ((SEP_REFINE (P * SEP_T) ($=) (STATE m0_proj) s) /\
+    rel_sequence (NEXT_REL $= NextStateM0) seq  s /\
+    rel_sequence (NEXT_REL $= NextStateM0U) seq' s' /\
+    m0u_m0_non_r_eq uart_r s' s /\ ((seq i).count <= s.count + t) )==>   
+	m0u_m0_non_r_eq uart_r (seq' i) (seq i) /\
+	m0u_r_eq uart_r s' (seq' i)`;
+
+
+val m0_non_r_eq_exists_thm = prove(``!s region.?s'. m0_non_r_eq region s s'``,
+     METIS_TAC [m0_non_r_eq_refl_thm]
+);
+
+   (** third attempt with stronger induction assumption **) 
+val NIT_COSIM_thm = Q.store_thm ("NIT_COSIM_thm", 
+    `!P t.  ((NIT uart_r P t) /\ (NEX P t)) ==> (COSIM P t)`, 
+    SIMP_TAC std_ss [ COSIM_def, PULL_FORALL]>>
+    (* Strengthen induction hypothesis  *)
+    `!P t s s' s_hat seq seq'  seq_hat i .
+        (m0_non_r_eq uart_r s s') /\
+	NIT uart_r P t /\
+	NEX P t ==>
+	SEP_REFINE (P * SEP_T) $= (STATE m0_proj) s /\
+	rel_sequence (NEXT_REL $= NextStateM0) seq s /\
+	rel_sequence (NEXT_REL $= NextStateM0) seq' s' /\
+	rel_sequence (NEXT_REL $= NextStateM0U) seq_hat s_hat /\
+	m0u_m0_non_r_eq uart_r s_hat s /\ (seq i).count <= s.count + t ==>
+        m0_non_r_eq uart_r (seq i) (seq' i) /\
+        m0_r_eq uart_r s' (seq' i) /\
+	m0u_m0_non_r_eq uart_r (seq_hat i) (seq i) /\
+	m0u_r_eq uart_r s_hat (seq_hat i) ` suffices_by(
+            METIS_TAC [m0_non_r_eq_exists_thm, SEQUENCE_EXISTS_THM]
+    )>>
+    REPEAT GEN_TAC>>
+    Induct_on `i`>-(   
+        `s.count <= s.count +t` by DECIDE_TAC>>
+	METIS_TAC [m0u_m0_non_r_eq_def, m0u_r_eq_refl_thm,
+                   m0_r_eq_refl_thm , rel_sequence_def]
+    )>>
+    STRIP_TAC>>STRIP_TAC>>
+    `(seq i).count <= s.count + t ` by (
+	(MP_TAC o Q.SPECL [`s`,`i`, `SUC i`, `seq`]) SEQ_MONO_B >>
+	ASM_SIMP_TAC std_ss []>>
+	DECIDE_TAC)>>
+    FULL_SIMP_TAC std_ss []>>
+    
+    Q.PAT_ASSUM `NIT uart_r _ _` (MP_TAC o Q.SPECL [`s`, `s'`, `seq`, `seq'`, `SUC i`]
+                                           o SIMP_RULE std_ss [ NIT_def])>>
+    FULL_SIMP_TAC std_ss []>>
+    STRIP_TAC >>
+
+    (* should get from from NEX: *)
+
+     `(seq(SUC i) = Next (seq(i))) /\ ((Next (seq i)).exception = NoException)` by (
+	Q.PAT_X_ASSUM `NIX P t` (
+            MP_TAC o Q.SPECL [`s`, `seq`, `SUC i`] o
+	    REWRITE_RULE [NEX_def])>>
+	FULL_SIMP_TAC (std_ss++LET_ss) [
+	    rel_sequence_def, NEXT_REL_EQ,
+            NextStateM0_def]>>
+        METIS_TAC []  
+      )>>
+   
+      
+
+    `(seq'(SUC i) = Next (seq'(i))) ` by(
+     `((seq' (SUC i)).exception = NoException)` by  FULL_SIMP_TAC std_ss[m0_non_r_eq_def]>>
+	FULL_SIMP_TAC (std_ss++LET_ss) [
+	    rel_sequence_def, NEXT_REL_EQ,
+            NextStateM0_def]>>
+	Cases_on  `(Next (seq' i)).exception = NoException`>- (
+	    METIS_TAC [])>>
+	Q.PAT_ASSUM `!n.
+		if (Next (seq' n)).exception = NoException then
+		    Next (seq' n) = seq' (SUC n)
+		else seq' (SUC n) = seq' n` (MP_TAC o Q.SPECL [`i`])>>
+	`(seq i).count = (Next(seq i)).count` suffices_by (
+	    (MP_TAC o Q.SPEC `seq (i:num)`) NEXT_MONO>>
+	    ASM_SIMP_TAC arith_ss [])>>
+	FULL_SIMP_TAC std_ss [m0_non_r_eq_def] >>
+	METIS_TAC[]
+    )>>
+    FULL_SIMP_TAC std_ss []>>
+
+    (* from NIT_STEP_thm and 16, 12, 13 *)
+    `NIT_STEP uart_r (seq i)`  suffices_by cheat
+    
+    ASM_SIMP_TAC std_ss  [NIT_STEP_thm, m0_non_r_eq_antisym_thm, m0_non_r_eq_trans_thm, m0_r_eq_trans_thm, m0_r_eq_antisym_thm]
+    
+    DB.find "NIT_STEP_thm"
+    SIMP_RULE std_ss [PULL_FORALL] NIT_STEP_thm
+    
+    (MP_TAC o Q.SPECL [`seq (i:num)`, `seq_hat (i:num)`]) AXI>>
+    ASM_SIMP_TAC std_ss [NIT_STEP_def, NIT_STEP_from_def]>> 
+DB.find "NIT_STEP_from"
+    
+    (* uart does not change, so uart is still predictable *)
+    `seq_hat(SUC i) = m0u_Next (seq_hat i)` by cheat>>
+    METIS_TAC [m0u_r_eq_trans_thm,  m0u_r_eq_antisym_thm]
+);
+
+    
+
+(********************************************)
+(*          Transfere properties            *)
+(*                                          *)
+(********************************************)
+
+
+
+val TP_def = Q.store_thm(
+    "TP_def",
+    `!P C Q c t. (SPEC M0_MODEL (P*m0_count c) C (Q*m0_count (c+t))) /\ 
+	(COSIM P t) /\  
+
+(!SET. P SET==>  DISJOINT SET UART) /\
+(!SET. Q SET==>  DISJOINT SET UART) ==>
+
+ 
+	    (SPEC M0U_MODEL (TO_M0U_PROP (P*m0_count c)) C (TO_M0U_PROP(Q*m0_count (c+t))))`,
+    cheat);
+
+val WS_COSIM_thm = Q.store_thm("WS_COSIM_thm",
+    `!P P' t t'. COSIM P t /\ t' < t  /\ (SEP_IMP P' P) ==> COSIM P' t'`,
+    SIMP_TAC arith_ss [COSIM_def, PULL_FORALL]>>
+    REPEAT STRIP_TAC>>(
+	Q.PAT_X_ASSUM `!s s' seq seq' i F._` (MP_TAC o Q.SPECL [`s`, `s'`, `seq`, `seq'`, `i`, `F'`] )>>
+	REPEAT STRIP_TAC>>
+	` (seq i).count ≤ t` by DECIDE_TAC>>
+	`SEP_REFINE (P * F') $= (STATE m0_proj) s` by (
+	REV_FULL_SIMP_TAC std_ss [SEP_IMP_def, STAR_def,SEP_REFINE_def]>>
+	METIS_TAC [])>>
+	METIS_TAC []
+    )
+);
+
+
+val _ = export_theory();
